theories/AD.v
@@ -36,7 +36,7 @@ Proof. intros. unfold Ddiv. rewrite real_mul, real_Dinv. reflexivity. Qed.
 (* Single-variable expression language *)
 Inductive Expr : Set :=
 | Const (s : S)
-| Var
+| Var   (i : nat)
 | Add   (e1 e2 : Expr)
 | Sub   (e1 e2 : Expr)
 | Mul   (e1 e2 : Expr)
@@ -44,10 +44,10 @@ Inductive Expr : Set :=
 | Div   (e1 e2 : Expr).
 
 (* Evaluation over the base field *)
-Fixpoint eval (e : Expr) (x : S) : S :=
+Fixpoint eval (e : Expr) (x : nat -> S) : S :=
     match e with
     | Const c   => c
-    | Var       => x
+    | Var i     => x i
     | Add e1 e2 => (eval e1 x + eval e2 x)%S
     | Sub e1 e2 => (eval e1 x - eval e2 x)%S
     | Mul e1 e2 => (eval e1 x * eval e2 x)%S
@@ -56,10 +56,10 @@ Fixpoint eval (e : Expr) (x : S) : S :=
     end.
 
 (* Evaluation over the duals *)
-Fixpoint eval_dual (e : Expr) (x : D) : D :=
+Fixpoint eval_dual (e : Expr) (x : nat -> D) : D :=
     match e with
     | Const c   => inj c
-    | Var       => x
+    | Var i     => x i
     | Add e1 e2 => Dual.add (eval_dual e1 x) (eval_dual e2 x)
     | Sub e1 e2 => Dual.sub (eval_dual e1 x) (eval_dual e2 x)
     | Mul e1 e2 => Dual.mul (eval_dual e1 x) (eval_dual e2 x)
@@ -97,25 +97,25 @@ Fixpoint eval_dual (e : Expr) (x : D) : D :=
     derivative (Div e1 e2)
         (Div (Sub (Mul de1 e2) (Mul e1 de2)) (Mul e2 e2)). *)
 
-Fixpoint deriv (e : Expr) : Expr :=
+Fixpoint deriv (e : Expr) (v : nat -> S) : Expr :=
     match e with
     | Const _   => Const 0%S
-    | Var       => Const 1%S
-    | Add e1 e2 => Add (deriv e1) (deriv e2)
-    | Sub e1 e2 => Sub (deriv e1) (deriv e2)
-    | Mul e1 e2 => Add (Mul (deriv e1) e2) (Mul e1 (deriv e2))
-    | Opp e1    => Opp (deriv e1)
+    | Var j     => Const (v j)
+    | Add e1 e2 => Add (deriv e1 v) (deriv e2 v)
+    | Sub e1 e2 => Sub (deriv e1 v) (deriv e2 v)
+    | Mul e1 e2 => Add (Mul (deriv e1 v) e2) (Mul e1 (deriv e2 v))
+    | Opp e1    => Opp (deriv e1 v)
     | Div e1 e2 =>
         (* (e1' e2 - e1 e2') / e2^2 *)
-        Div (Sub (Mul (deriv e1) e2) (Mul e1 (deriv e2)))
+        Div (Sub (Mul (deriv e1 v) e2) (Mul e1 (deriv e2 v)))
             (Mul e2 e2)
     end.
 
 (* Well-definedness: Every denominator is nonzero *)
-Fixpoint defined_at (e : Expr) (x : S) : Prop :=
+Fixpoint defined_at (e : Expr) (x : nat -> S) : Prop :=
     match e with
     | Const _   => True
-    | Var       => True
+    | Var _     => True
     | Add e1 e2 => defined_at e1 x /\ defined_at e2 x
     | Sub e1 e2 => defined_at e1 x /\ defined_at e2 x
     | Mul e1 e2 => defined_at e1 x /\ defined_at e2 x
@@ -125,44 +125,46 @@ Fixpoint defined_at (e : Expr) (x : S) : Prop :=
 
 (* Correctness
 
-   After evaluating [e] over the duals at [a + eps], its real part
-   is [eval e a], and its dual part is [eval (deriv e) a]. *)
+   Evaluating an expression [e] over multivariate dual numbers gives two results:
+   1. The real part is the standard evaluation of the expression
+   2. The dual part is the partial derivative with respect to variable [i]. *)
 Theorem eval_dual_correct :
-    forall e a,
+    forall (e : Expr) (a : nat -> S) (v : nat -> S),
+        let env : nat -> D := fun j => (a j, v j) in
         defined_at e a ->
-        real (eval_dual e (a, 1%S)) = eval e a /\
-        du (eval_dual e (a, 1%S))   = eval (deriv e) a.
+        real (eval_dual e env) = eval e a /\
+        du (eval_dual e env)   = eval (deriv e v) a.
 Proof.
-    induction e; intros a Hdef; cbn in Hdef.
+    induction e; cbv zeta; intros a v Hdef; cbn in Hdef.
     - (* Const c *)
       cbn. unfold inj. now split.
     - (* Var *)
       cbn. now split.
     - (* Add e1 e2 *)
       destruct Hdef as [H1 H2].
-      destruct (IHe1 a H1) as [Hr1 Hd1].
-      destruct (IHe2 a H2) as [Hr2 Hd2].
+      destruct (IHe1 a v H1) as [Hr1 Hd1].
+      destruct (IHe2 a v H2) as [Hr2 Hd2].
       cbn. rewrite Hr1, Hr2, Hd1, Hd2. now split.
     - (* Sub e1 e2 *)
       destruct Hdef as [H1 H2].
-      destruct (IHe1 a H1) as [Hr1 Hd1].
-      destruct (IHe2 a H2) as [Hr2 Hd2].
+      destruct (IHe1 a v H1) as [Hr1 Hd1].
+      destruct (IHe2 a v H2) as [Hr2 Hd2].
       cbn. unfold Dual.sub.
       rewrite Hr1, Hr2, Hd1, Hd2.
       split; ring.
     - (* Mul e1 e2 *)
       destruct Hdef as [H1 H2].
-      destruct (IHe1 a H1) as [Hr1 Hd1].
-      destruct (IHe2 a H2) as [Hr2 Hd2].
+      destruct (IHe1 a v H1) as [Hr1 Hd1].
+      destruct (IHe2 a v H2) as [Hr2 Hd2].
       cbn. rewrite Hr1, Hr2, Hd1, Hd2.
       split; ring.
     - (* Opp e1 *)
-      destruct (IHe a Hdef) as [Hr Hd].
+      destruct (IHe a v Hdef) as [Hr Hd].
       cbn. rewrite Hr, Hd. split; ring.
     - (* Div e1 e2 *)
       destruct Hdef as [H1 [H2 Hnz]].
-      destruct (IHe1 a H1) as [Hr1 Hd1].
-      destruct (IHe2 a H2) as [Hr2 Hd2].
+      destruct (IHe1 a v H1) as [Hr1 Hd1].
+      destruct (IHe2 a v H2) as [Hr2 Hd2].
       cbn. split.
       + rewrite Hr1, Hr2.
         symmetry. apply div_def.
